userspace/include/portlib.h
@@ -1,0 +1,8 @@
+#ifndef _PORTLIB_H_
+#define _PORTLIB_H_
+
+#include <stdarg.h>
+#include <u.h>
+#include <libc.h>
+
+#endif
