userspace/include/stdint.h
@@ -1,0 +1,14 @@
+#ifndef _STDINT_H
+#define _STDINT_H
+#include <u.h>
+typedef u8int uint8_t;
+typedef u16int uint16_t;
+typedef u32int uint32_t;
+typedef u64int uint64_t;
+typedef s8int int8_t;
+typedef s16int int16_t;
+typedef s32int int32_t;
+typedef s64int int64_t;
+typedef uintptr uintptr_t;
+typedef intptr intptr_t;
+#endif
