userspace/include/sys/types.h
@@ -1,0 +1,10 @@
+#ifndef _SYS_TYPES_H
+#define _SYS_TYPES_H
+#include <u.h>
+typedef ssize ssize_t;
+// size_t is usually in stddef.h, but if missing:
+#ifndef _SIZE_T
+#define _SIZE_T
+typedef usize size_t;
+#endif
+#endif
