userspace/include/u.h
@@ -1,0 +1,55 @@
+/* Plan 9 universal header */
+#ifndef _U_H_
+#define _U_H_
+
+#ifndef static_assert
+# if defined(__STDC_VERSION__) && __STDC_VERSION__ >= 201112L
+#  define static_assert _Static_assert
+# elif defined(__cplusplus) && __cplusplus >= 201103L
+#  define static_assert(x, msg) static_assert(x, msg)
+# else
+#  define static_assert(x, msg) typedef char static_assert_##msg[(x)?1:-1]
+# endif
+#endif
+
+#ifndef _Noreturn
+#define _Noreturn __attribute__((noreturn))
+#endif
+
+typedef unsigned char uchar;
+typedef unsigned short ushort;
+typedef unsigned int uint;
+typedef unsigned long ulong;
+typedef unsigned long long uvlong;
+typedef long long vlong;
+
+typedef unsigned long usize;
+typedef long ssize;
+typedef unsigned long uintptr;
+typedef long intptr;
+
+/* Plan 9 fixed-width types */
+typedef unsigned char u8int;
+typedef unsigned short u16int;
+typedef unsigned int u32int;
+typedef unsigned long long u64int;
+typedef signed char s8int;
+typedef signed short s16int;
+typedef signed int s32int;
+typedef signed long long s64int;
+
+typedef u32int Rune;	/* UTF-8 code point */
+
+#define nelem(x) (sizeof(x)/sizeof((x)[0]))
+#ifndef offsetof
+#define offsetof(s, m) (ulong)(&(((s*)0)->m))
+#endif
+
+#define nil ((void*)0)
+
+/* USED macro to suppress unused warnings */
+#define USED(...) if(__VA_ARGS__){}
+
+typedef long jmp_buf[10];
+
+#endif /* _U_H_ */
