userspace/libc/errstr.c
@@ -1,0 +1,23 @@
+#include <u.h>
+#include <libc.h>
+#include <sys.h>
+#include "syscall.h"
+#include "syscall_ops.h"
+
+int
+errstr(char *buf, uint nbuf)
+{
+	return (int)syscall3(ERRSTR, (long)buf, nbuf, 0);
+}
+
+void
+werrstr(char *fmt, ...)
+{
+	char buf[ERRMAX];
+	va_list arg;
+
+	va_start(arg, fmt);
+	vsnprint(buf, sizeof buf, fmt, arg);
+	va_end(arg);
+	errstr(buf, sizeof buf);
+}
